Modify the semantics of case
The case expression clause selection is modified:
The clause 'cl' will be evaluated, if:
 - Its pattern matches the value
 - Its guard evaluates to 'true' in the extended environment
 - For every clause 'cl_0' before 'cl' either:
   - The pattern of 'cl_0' does not match the value OR
   - The guard of 'cl_0' evaluates to 'false' in the extended
   environment

For this purpose the index_case_equality lemma was defined.

Add an additional example for case expression.

Simplify proofs with the determinism_hypo helper proposition.
Modify the determinism of case according to the modifications.

Core_Erlang_Helpers.v
@@ -247,13 +247,21 @@ with match_and_bind_elements (exps : list Expression) (t : Tuple) (pf : forall e
   end
 .
 
+Fixpoint match_clause (e : Value) (cls : list Clause) (i : nat) : option (Expression * Expression * list (Var * Value)) :=
+match cls, i with
+| [], _ => None
+| ((CCons p g exp)::xs), 0 => if match_expression_to_pattern (proj1_sig e) p (proj2_sig e) then Some (g, exp, (match_expression_bind_pattern (proj1_sig e) p (proj2_sig e))) else None
+| ((CCons p g exp)::xs), S n' => match_clause e xs n'
+end
+.
+
 (* Get the matching clause to an Expression *)
-Fixpoint match_clauses (e : Value) (cls : list Clause) : option (Expression * Expression * list (Var * Value)) :=
+(* Fixpoint match_clauses (e : Value) (cls : list Clause) : option (Expression * Expression * list (Var * Value)) :=
 match cls with
 | [] => None
 | ((CCons p g exp)::xs) => if match_expression_to_pattern (proj1_sig e) p (proj2_sig e) then Some (g, exp, (match_expression_bind_pattern (proj1_sig e) p (proj2_sig e))) else match_clauses e xs
 end
-.
+.*)
 
 Fixpoint correct_clauses (cl : list Clause) : bool :=
 match cl with
